WIP

ems/ModSemE.v
@@ -16,7 +16,6 @@ Section EVENTSCOMMON.
   | Choose (X: Type): eventE X
   | Take X: eventE X
   | Syscall (fn: gname) (args: Any.t) (rvs: Any.t -> Prop): eventE Any.t
-  | Spwan_t (mn: option mname) (fn: gname) (args: Any.t): eventE nat
   .
 
   (* Notation "'Choose' X" := (trigger (Choose X)) (at level 50, only parsing). *)
@@ -124,7 +123,7 @@ Section EVENTSL.
   .
 
   Inductive schE: Type -> Type :=
-  | Spwan (mn: option mname) (fn: gname) (args: Any.t): schE nat
+  | Spawn (mn: mname) (fn: gname) (args: Any.t): schE nat
   | Yield: schE unit
   .
 
@@ -154,103 +153,118 @@ Section EVENTSL.
   (********************************************************************)
   (*************************** Interpretation *************************)
   (********************************************************************)
-  
-  Definition interp_schE_aux {R} :
-    itree Es R -> itree (callE +' pE +' eventE) ((itree Es R) + R).
-  Proof.
-    eapply ITree.iter.
-    intros itr.
-    apply observe in itr; destruct itr as [r | itr | X e k].
-    - (* Ret *)
-      exact (Ret (inr (inr r))).
-    - (* Tau *)
-      exact (Ret (inl itr)).
-    - (* Vis *)
-      destruct e as [|[|[]]].
-      + (* schE *)
-        destruct s.
-        * (* Spwan *)
-          exact (Vis (inr1 (inr1 (Spwan_t mn fn args))) (fun x => Ret (inl (k x)))).
-        * (* Yield *)
-          exact (Ret (inr (inl (k tt)))).
-      + (* callE *)
-        exact (Vis (inl1 c) (fun x => Ret (inl (k x)))).
-      + (* pE *)
-        exact (Vis (inr1 (inl1 p)) (fun x => Ret (inl (k x)))).
-      + (* eventE *)
-        exact (Vis (inr1 (inr1 e)) (fun x => Ret (inl (k x)))).
-  Defined.
+  Section Scheduler.
+    Definition interp_schE_aux {R} :
+      itree Es R -> itree (callE +' pE +' eventE) ((itree Es R) + R).
+    Proof.
+      eapply ITree.iter.
+      intros itr.
+      apply observe in itr; destruct itr as [r | itr | X e k].
+      - (* Ret *)
+        exact (Ret (inr (inr r))).
+      - (* Tau *)
+        exact (Ret (inl itr)).
+      - (* Vis *)
+        destruct e as [|[|[]]].
+        + (* schE *)
+          destruct s.
+          * (* Spawn *)
+            exact (Vis (inr1 (inr1 (Spawn_t fn args))) (fun x => Ret (inl (k x)))).
+          * (* Yield *)
+            exact (Ret (inr (inl (k tt)))).
+        + (* callE *)
+          exact (Vis (inl1 c) (fun x => Ret (inl (k x)))).
+        + (* pE *)
+          exact (Vis (inr1 (inl1 p)) (fun x => Ret (inl (k x)))).
+        + (* eventE *)
+          exact (Vis (inr1 (inr1 e)) (fun x => Ret (inl (k x)))).
+    Defined.
 
-  Variant schedulerE (RT : Type) : Type -> Type :=
-  | Execute : thread_id -> schedulerE RT (option RT)
-  .
-  
-  Notation threads RT := (alist thread_id (itree Es RT)).
-  Notation tids := (alist thread_id unit).
-  Definition scheduler RT R := itree (schedulerE RT +' eventE) R.
+    Variant schedulerE (RT : Type) : Type -> Type :=
+      | Execute : thread_id -> schedulerE RT (option RT).
+    
+    Notation threads RT := (alist thread_id (itree Es RT)).
+    Notation tids := (alist thread_id unit).
+    Definition scheduler RT R := itree (schedulerE RT +' eventE) R.
 
-  Definition new_itr (RT: Type) (r: RT) mn fn args: itree Es RT :=
-    v <- trigger (Call mn fn args);;
-    Ret r.
-  
-  Definition interp_sched RT R : threads RT * thread_id * scheduler RT R -> itree (callE +' pE +' eventE) R.
-  Proof.
-    eapply ITree.iter. intros [[ts max_tid] sch].
-    destruct (observe sch) as [r | sch' | X [e|e] ktr].
-    - exact (Ret (inr r)).
-    - exact (Ret (inl (ts, max_tid, sch'))).
-    - destruct e.
-      destruct (alist_find n ts) as [t|].
-      * exact (r <- interp_schE_aux t;;
-               match r with
-               | inl t' => Ret (inl (alist_add n t' ts, max_tid, ktr None))
-               | inr r => Ret (inl (alist_remove n ts, max_tid, ktr (Some r)))
-               end).
-      * exact triggerUB.
-    - destruct e.
-      * (* Choose *)
-        exact (Vis (inr1 (inr1 (Choose X))) (fun x => Ret (inl (ts, max_tid, ktr x)))).
-      * (* Take *)
-        exact (Vis (inr1 (inr1 (Take X))) (fun x => Ret (inl (ts, max_tid, ktr x)))).
-      * (* Syscall *)
-        exact (Vis (inr1 (inr1 (Syscall fn args rvs))) (fun x => Ret (inl (ts, max_tid, ktr x)))).
-      * (* Spwan *)
-        (* remember (ITree.trigger (subevent RT (Call mn fn args))) as new_itr. *)
-        (* remember (trigger (Call mn fn args)) as new_itr2. *)
-        (* exact (Ret (inl (alist_add max_tid new_itr ts, max_tid + 1, ktr max_tid))). *)
-        exact (Vis (inr1 (inr1 (Spwan_t mn fn args))) (fun x => Ret (inl (ts, max_tid, ktr x)))).
-  Defined.
+    Definition new_itr {RT: Type} fn args : itree Es RT :=
+      v <- ITree.trigger (inr1 (inl1 (Call None fn args)));;
+      triggerNB.
+    
+    Definition interp_sched RT R : threads RT * thread_id * scheduler RT R -> itree (callE +' pE +' eventE) R.
+    Proof.
+      eapply ITree.iter. intros [[ts max_tid] sch].
+      destruct (observe sch) as [r | sch' | X [e|e] ktr].
+      - exact (Ret (inr r)).
+      - exact (Ret (inl (ts, max_tid, sch'))).
+      - destruct e.
+        destruct (alist_find n ts) as [t|].
+        * exact (r <- interp_schE_aux t;;
+                 match r with
+                 | inl t' => Ret (inl (alist_add n t' ts, max_tid, ktr None))
+                 | inr r => Ret (inl (alist_remove n ts, max_tid, ktr (Some r)))
+                 end).
+        * exact triggerUB.
+      - destruct e.
+        * (* Choose *)
+          exact (Vis (inr1 (inr1 (Choose X))) (fun x => Ret (inl (ts, max_tid, ktr x)))).
+        * (* Take *)
+          exact (Vis (inr1 (inr1 (Take X))) (fun x => Ret (inl (ts, max_tid, ktr x)))).
+        * (* Syscall *)
+          exact (Vis (inr1 (inr1 (Syscall fn args rvs))) (fun x => Ret (inl (ts, max_tid, ktr x)))).
+        * (* Spawn_t *)
+          exact (Ret (inl (alist_add max_tid (new_itr fn args) ts, max_tid + 1, ktr max_tid))).
+    Defined.
 
-  Definition sched_nondet_body {R} q tid r : scheduler R (thread_id * tids + R) :=
-    match r with
-    | None =>
-        tid' <- ITree.trigger (inr1 (Choose thread_id));;
-        match alist_pop tid' (alist_add tid tt q) with
-        | None => triggerNB
-        | Some (_, q') => Ret (inl (tid', q'))
-        end
-    | Some r =>
-        if true
-        then Ret (inr r)
-        else
+    Definition sched_nondet_body {R} q tid r : itree eventE (thread_id * tids + R) :=
+      match r with
+      | None =>
           tid' <- ITree.trigger (inr1 (Choose thread_id));;
-          match alist_pop tid' q with
+          match alist_pop tid' (alist_add tid tt q) with
           | None => triggerNB
           | Some (_, q') => Ret (inl (tid', q'))
           end
-    end.
+      (* | spawn *)
+      | Some r =>
+          if true (* TODO *)
+          then Ret (inr r)
+          else
+            tid' <- ITree.trigger (inr1 (Choose thread_id));;
+            match alist_pop tid' q with
+            | None => triggerNB
+            | Some (_, q') => Ret (inl (tid', q'))
+            end
+      end.
 
-  Definition sched_nondet R0 : thread_id * tids -> scheduler R0 R0 :=
-    ITree.iter (fun '(tid, q) =>
-                  r <- ITree.trigger (inl1 (Execute _ tid));;
-                  sched_nondet_body q tid r).
+    Definition sched_nondet R0 : thread_id * tids -> scheduler R0 R0 :=
+      ITree.iter (fun '(tid, q) =>
+                    r <- ITree.trigger (inl1 (Execute _ tid));;
+                    sched_nondet_body q tid r).
 
-  Definition alist_key_set K V (t: alist K V): alist K unit :=
-    List.map (fun x => (fst x, tt)) t.
+    Definition alist_key_set K V (t: alist K V): alist K unit :=
+      List.map (fun x => (fst x, tt)) t.
 
-  Definition interp_schE
-    R ths tid : itree (callE +' pE +' eventE) R :=
-    interp_sched (ths, 1, sched_nondet _ (tid, alist_remove tid (alist_key_set ths))).
+    Definition interp_schE
+      R ths tid max_tid : itree (callE +' pE +' eventE) R :=
+      interp_sched (ths, max_tid, sched_nondet _ (tid, alist_remove tid (alist_key_set ths))).
+  End Scheduler.
+
+  (* Section Sch_example. *)
+  (*   Definition f x : itree Es Any.t := *)
+  (*     y <- trigger (Call None "g" [x - 1]↑);; *)
+  (*     y <- y↓?;; *)
+  (*     Ret (x + y)↑. *)
+    
+  (*   Definition g x : itree Es Any.t := *)
+  (*     y <- trigger (Call None "f" [x - 1]↑);; *)
+  (*     y <- y↓?;; *)
+  (*     Ret (x + y)↑. *)
+
+  (*   Definition main : itree Es Any.t := *)
+  (*     a <- trigger (Call None "f" [4]↑);; *)
+  (*     Ret a. *)
+                        
+  (* End Sch_example. *)
 
   Definition handle_pE {E}: pE ~> stateT p_state (itree E) :=
     fun _ e mps =>
@@ -266,7 +280,7 @@ Section EVENTSL.
   (*   interp_pE (interp_rE (interp_mrec prog itr0) rst0) pst0 *)
   (* . *)
   Definition interp_Es A (prog: callE ~> itree (callE +' pE +' eventE)) (itr0: itree Es A) (st0: p_state): itree eventE (p_state * _)%type :=
-    '(st1, v) <- interp_pE (interp_mrec prog (interp_schE (alist_add 0 itr0 []) 0)) st0;;
+    '(st1, v) <- interp_pE (interp_mrec prog (interp_schE (alist_add 0 itr0 []) 0 1)) st0;;
     Ret (st1, v)
   .
 
